src/Spec/AbstractionSpec.v
@@ -1,0 +1,112 @@
+Require Import Spec.Proc.
+Require Import Spec.Hoare.
+
+Require Import Helpers.RelationAlgebra.
+Require Import Helpers.RelationRewriting.
+Require Import Abstraction.
+
+Section Abstraction.
+  Context (AState CState:Type).
+  Context (absr: relation AState CState unit).
+
+  (* define refinement as transforming an abstract specification to a concrete
+  one (a program satisfying the abstract spec should satisfy the concrete spec
+  after refinement-preserving compilation) *)
+  Definition refine_spec T R (spec: Specification T R AState)
+    : AState -> Specification T R CState :=
+    fun s cs =>
+      {| pre := absr s cs tt /\
+                (spec s).(pre);
+         post := fun cs' r =>
+                   exists s', absr s' cs' tt /\
+                         (spec s).(post) s' r;
+         alternate := fun cs' r =>
+                        exists s', absr s' cs' tt /\
+                              (spec s).(alternate) s' r; |}.
+
+  Context A_Op C_Op `(a_sem: Dynamics A_Op AState) `(c_sem:Dynamics C_Op CState).
+
+  Import RelationNotations.
+
+  Lemma proc_rspec_refine_exec T R (p: proc C_Op T) (rec: proc C_Op R) spec:
+    (forall t, proc_rspec (c_sem) p rec (refine_spec spec t)) ->
+    (forall sA sC, absr sA sC tt -> (spec sA).(pre)) ->
+    _ <- absr; exec (c_sem) p ---> v <- spec_exec (spec); _ <- absr; pure v.
+  Proof.
+    intros Hprspec Habstr_pre.
+    intros sA sC b ([]&sTstart&Hrd&Hexec).
+    destruct (Hprspec sA).
+    eapply H in Hexec. simpl in Hexec.
+    clear -Hrd Hexec Habstr_pre.
+    edestruct Hexec; eauto. simpl. intuition; eauto.
+    do 2 eexists; intuition.
+    * intros ?; eauto.
+    * firstorder.
+  Qed.
+
+  Lemma proc_rspec_refine_rec T R (p: proc C_Op T) (rec: proc C_Op R) spec:
+    (forall t, proc_rspec (c_sem) p rec (refine_spec spec t)) ->
+    (forall sA sC, absr sA sC tt -> (spec sA).(pre)) ->
+    _ <- absr; rexec (c_sem) p rec ---> v <- spec_aexec spec; _ <- absr; pure v.
+  Proof.
+    intros Hprspec Habstr_pre.
+    intros sA sC b ([]&sTstart&Hrd&Hexec).
+    destruct (Hprspec sA).
+    eapply H0 in Hexec. simpl in Hexec.
+    clear -Hrd Hexec Habstr_pre.
+    edestruct Hexec; eauto. simpl. intuition; eauto.
+    do 2 eexists; intuition.
+    * intros ?; eauto.
+    * firstorder.
+  Qed.
+
+  Lemma proc_rspec_crash_refines T (p: proc C_Op T) (rec: proc C_Op unit)
+        spec op:
+    (forall t, proc_rspec c_sem p rec (refine_spec spec t)) ->
+    (forall sO sT, absr sO sT tt -> (spec sO).(pre)) ->
+    (spec_exec (spec) ---> exec a_sem (Prim op)) ->
+    (spec_aexec (spec) --->
+                  (a_sem.(crash_step) + (a_sem.(step) op;; a_sem.(crash_step)))) ->
+    crash_refines absr c_sem p rec (a_sem.(step) op)
+                  (a_sem.(crash_step) + (a_sem.(step) op;; a_sem.(crash_step))).
+  Proof.
+    intros ?? He Ha. unfold crash_refines, refines. split.
+    - setoid_rewrite <-He. eapply proc_rspec_refine_exec; eauto.
+    - setoid_rewrite <-Ha. eapply proc_rspec_refine_rec; eauto.
+  Qed.
+
+  Lemma proc_rspec_crash_refines_op T (p: proc C_Op T) (rec: proc C_Op unit)
+        spec (op: A_Op T):
+    (forall t, proc_rspec c_sem p rec (refine_spec spec t)) ->
+    (forall sA sC, absr sA sC tt -> (spec sA).(pre)) ->
+    (forall sA sC sA' v, absr sA' sC tt -> (spec sA).(post) sA' v
+                         -> (op_cstep_spec a_sem op sA).(post) sA' v) ->
+    (forall sA sC sA' v, absr sA sC tt -> (spec sA).(alternate) sA' v
+                         -> (op_cstep_spec a_sem op sA).(alternate) sA' v) ->
+    crash_refines absr c_sem p rec (a_sem.(step) op)
+                  (a_sem.(crash_step) + (a_sem.(step) op;; a_sem.(crash_step))).
+  Proof.
+    intros Hprspec Hpre Hpost Halt. unfold crash_refines, refines; split.
+    - setoid_rewrite <-op_cstep_spec_complete1.
+      unfold spec_exec.
+      intros sA sC' t Hl.
+      destruct Hl as ([]&sC&?&Hexec).
+      eapply (Hprspec sA) in Hexec.
+      simpl in Hexec. edestruct Hexec as (sA'&?&?); eauto.
+      { unfold refine_spec; simpl. split; auto. eapply Hpre; eauto. }
+      exists t, sA'; split; auto.
+      * intros Hpre'. eapply Hpost; eauto.
+      * exists tt, sC'; firstorder.
+    - setoid_rewrite <-op_cstep_spec_complete2.
+      unfold spec_aexec.
+      intros sA sC' [] Hl.
+      destruct Hl as ([]&sC&?&Hexec).
+      eapply (Hprspec sA) in Hexec.
+      simpl in Hexec. edestruct Hexec as (sA'&?&?); eauto.
+      { unfold refine_spec; simpl. split; auto. eapply Hpre; eauto. }
+      exists tt, sA'; split; auto.
+      * intros Hpre'. eapply Halt; eauto.
+      * exists tt, sC'; firstorder.
+  Qed.
+
+End Abstraction.
